verif/btrees/verif_splitnode_part0.v
@@ -12,7 +12,6 @@ Require Import btrees.
 Require Import btrees_sep.
 Require Import btrees_spec.
 Require Import verif_newnode.
-Require Import verif_findindex.
 
 Lemma upd_Znth_twice: forall (A:Type) l i (x:A) x',
           0 <= i < Zlength l -> 
@@ -27,6 +26,29 @@ Proof.
   auto.
 Qed.
 
+(* Move to floyd *)
+Lemma Vptrofs_inj: forall key1 key2,
+    Vptrofs key1 = Vptrofs key2 ->
+    key1 = key2.
+Proof.
+intros.
+unfold Vptrofs in H.
+destruct Archi.ptr64 eqn:b.
+*
+assert (Ptrofs.to_int64 key1 = Ptrofs.to_int64 key2) by congruence.
+clear H.
+apply (f_equal Ptrofs.of_int64) in H0.
+rewrite ?Ptrofs.of_int64_to_int64 in H0 by auto.
+auto.
+*
+assert (Ptrofs.to_int key1 = Ptrofs.to_int key2) by congruence.
+apply (f_equal Ptrofs.of_int) in H0.
+rewrite ?Ptrofs.of_int_to_int in H0 by auto.
+auto.
+Qed.
+
+
+(*
 Lemma key_repr_k: forall key1 key2,
     Vptrofs key1 = Vptrofs key2 ->
     k_ key1 = k_ key2.
@@ -42,6 +64,7 @@ Proof.
   rewrite <- ?int_unsigned_ptrofs_toint by auto.
   f_equal; auto.
 Qed.
+*)
 
 Lemma Some_inj: forall A (a:A) b, Some a = Some b -> a = b.
 Proof.
@@ -67,7 +90,7 @@ subst.
 autorewrite with sublist in *.
 eauto.
 simpl in *.
-destruct (k_ k <=? k_ k0).
+destruct (negb (Ptrofs.ltu k0 k)).
 -
 clear - H H1 H2.
 destruct (zeq i 0).
@@ -112,7 +135,7 @@ rewrite Znth_map in H4 by omega.
 inv H4.
 generalize dependent i; induction H; intros.
 simpl in *.
-destruct (k_ k <=? k_ k0); autorewrite with sublist in *.
+destruct (negb (Ptrofs.ltu k0 k)); autorewrite with sublist in *.
 -
 destruct (zeq i 0).
 subst.
@@ -135,7 +158,7 @@ autorewrite with sublist in *.
 omega.
 -
 simpl in *.
-destruct (k_ k <=? k_ k0); autorewrite with sublist in *.
+destruct (negb (Ptrofs.ltu k0 k)); autorewrite with sublist in *.
 destruct (zeq i 0).
 subst.
 autorewrite with sublist. eauto.
@@ -176,7 +199,7 @@ Proof.
   induction le; intros.
   - simpl. auto.
   - simpl.
-     destruct (k_ key <=? k_ _). auto. rewrite IHle. auto.
+     destruct (negb (Ptrofs.ltu (entry_key a) key)). auto. rewrite IHle. auto.
 Qed.
 
 Lemma FRI_repr: forall X (le:list (entry X)) key1 key2 i,
@@ -186,7 +209,7 @@ Proof.
   intros. generalize dependent i. induction le; intros.
   - simpl. auto.
   - simpl. 
-    rewrite IHle. rewrite key_repr_k with (key2:=key2) by auto. auto.
+    rewrite IHle. apply Vptrofs_inj in H. subst key2. auto.
 Qed.
 
 Lemma FRI_bound:
@@ -197,7 +220,7 @@ intros.
 revert i; induction le; intros. simpl. list_solve.
 autorewrite with sublist.
 simpl.
-destruct (k_ key <=? k_ (entry_key a)).
+destruct (negb (Ptrofs.ltu (entry_key a) key)).
 rep_omega.
 specialize (IHle (Z.succ i)).
 omega.
@@ -224,7 +247,7 @@ Proof.
   - simpl in *. subst. autorewrite with sublist in H2. 
       autorewrite with sublist. auto.
   - simpl in *. autorewrite with sublist in H2.
-     destruct (k_ (entry_key e) <=? k_ _) eqn:?H;
+     destruct (negb (Ptrofs.ltu (entry_key a) (entry_key e))) eqn:?H;
         subst. autorewrite with sublist. auto.
         pose proof (FRI_increase X le (entry_key e) (Z.succ i)).
        pose proof (FRI_bound _ le (entry_key e) (Z.succ i)).
