verif/btrees/verif_splitnode_part4.v
@@ -208,8 +208,8 @@ Proof.
       LOCAL(temp _newNode vnewnode; temp _tgtIdx (Vint (Int.repr fri));
                  lvar _allEntries (tarray tentry 16) v_allEntries; temp _node nval; temp _entry pe)
      SEP(mem_mgr gv; btnode_rep nleft; btnode_rep (empty_node false false Last vnewnode);
-           data_at Ews tentry (Vptrofs (Ptrofs.repr (k_ k)), inl (getval ce)) pe;
-           data_at Tsh (tarray tentry 16) (map entry_val_rep (sublist 0 fri le)  ++ (Vptrofs (Ptrofs.repr (k_ k)), inl (getval ce)) :: map entry_val_rep (sublist fri i le) ++ ent_end) v_allEntries;
+           data_at Ews tentry (Vptrofs k, inl (getval ce)) pe;
+           data_at Tsh (tarray tentry 16) (map entry_val_rep (sublist 0 fri le)  ++ (Vptrofs k, inl (getval ce)) :: map entry_val_rep (sublist fri i le) ++ ent_end) v_allEntries;
            entry_rep(keychild val ke ce)))%assert.
 
     abbreviate_semax.
@@ -262,8 +262,8 @@ Proof.
       (* rewrite upd_Znth_app2. *)
       rewrite upd_Znth_same.
     set (fri := findRecordIndex n k) in *.
-      assert((upd_Znth (i + 1) (map entry_val_rep (sublist 0 fri le)  ++ (Vptrofs (Ptrofs.repr (k_ k)), inl (getval ce)) :: map entry_val_rep (sublist fri i le) ++ x) (Vptrofs ki, inl (getval ci))) 
-                 = (map entry_val_rep (sublist 0 fri le)  ++ (Vptrofs (Ptrofs.repr (k_ k)), inl (getval ce)) :: map entry_val_rep (sublist fri (i + 1) le) ++ sublist 1 (Zlength x) x)).
+      assert((upd_Znth (i + 1) (map entry_val_rep (sublist 0 fri le)  ++ (Vptrofs k, inl (getval ce)) :: map entry_val_rep (sublist fri i le) ++ x) (Vptrofs ki, inl (getval ci))) 
+                 = (map entry_val_rep (sublist 0 fri le)  ++ (Vptrofs k, inl (getval ce)) :: map entry_val_rep (sublist fri (i + 1) le) ++ sublist 1 (Zlength x) x)).
       { autorewrite with sublist. f_equal.
         change (?A::?B) with ([A]++B).
         rewrite upd_Znth_app2 by list_solve. simpl. f_equal.
@@ -279,6 +279,7 @@ Proof.
       }
       rewrite <- ?Vptrofs_repr_Vlong_repr by auto.
     change (Vlong (Ptrofs.to_int64 ki)) with (Vptrofs ki) in *.
+    change (Vlong (Ptrofs.to_int64 k)) with (Vptrofs k) in *.
       rewrite H18. simpl. cancel.
       list_solve.
       list_solve.
